OcapnLean.lean
@@ -10,6 +10,7 @@ import OcapnLean.Captp.Channels
 import OcapnLean.Captp.RefFifo
 import OcapnLean.Captp.RefFifoForwarding
 import OcapnLean.Captp.Impl.MultiVat
+import OcapnLean.Captp.Impl.PromiseForwarding
 import OcapnLean.Captp.RefinementMultiVat
 import OcapnLean.Captp.CrossedHellos
 import OcapnLean.Captp.Gc
